dsn/Lang/Dynamic/Convergent.lean
@@ -1,0 +1,37 @@
+import Lang.Basic
+import Lang.Dynamic.Transition
+import Lang.Dynamic.EvalCon
+import Lang.Dynamic.TransitionStar
+
+set_option pp.fieldNotation false
+
+
+namespace Lang.Dynamic
+
+def Convergent (e : Expr) : Prop :=
+  ∃ e' , TransitionStar e e' ∧ Expr.is_value e'
+
+mutual
+
+  theorem Convergent.subject_reduction
+    (transition : Transition e e')
+  : Convergent e → Convergent e'
+  := by sorry
+
+  theorem Convergent.subject_expansion
+    (transition : Transition e e')
+  : Convergent e' → Convergent e
+  := by sorry
+
+end
+
+
+theorem Convergent.evalcon_reflection :
+  EvalCon E →
+  Convergent (E e) →
+  Convergent e
+:= by
+  sorry
+
+
+end Lang.Dynamic
