dsn/Lang/Dynamic/Divergent.lean
@@ -1,0 +1,38 @@
+
+import Lang.Basic
+import Lang.Dynamic.Transition
+import Lang.Dynamic.EvalCon
+import Lang.Dynamic.TransitionStar
+
+set_option pp.fieldNotation false
+
+
+namespace Lang.Dynamic
+
+
+def Divergent (e : Expr) : Prop :=
+  (∀ e', TransitionStar e e' → ∃ e'' , Transition e' e'')
+
+
+mutual
+
+  theorem Divergent.subject_reduction
+    (transition : Transition e e')
+  : Divergent e → Divergent e'
+  := by sorry
+
+  theorem Divergent.subject_expansion
+    (transition : Transition e e')
+  : Divergent e' → Divergent e
+  := by sorry
+
+end
+
+theorem Divergent.evalcon_reflection :
+  EvalCon E →
+  Divergent (E e) →
+  Divergent e
+:= by
+  sorry
+
+end Lang.Dynamic
