dsn/Lang/Dynamic/EvalCon.lean
@@ -1,0 +1,90 @@
+import Lang.Basic
+import Lang.Dynamic.Transition
+
+set_option pp.fieldNotation false
+
+namespace Lang.Dynamic
+
+
+inductive EvalCon : (Expr → Expr) → Prop
+| hole : EvalCon (fun e => e)
+| applicator e' : EvalCon E → EvalCon (fun e => .app (E e) e')
+| applicand f : EvalCon E → EvalCon (fun e => .app (.function f) (E e))
+
+
+theorem EvalCon.soundness
+  (evalcon : EvalCon E)
+  (transition : Transition e e')
+: Transition (E e) (E e')
+:= by induction evalcon with
+| hole =>
+  simp
+  exact transition
+| applicator arg evalcon' ih =>
+  simp
+  apply Transition.applicator
+  exact ih
+| applicand f evalcon' ih =>
+  simp
+  apply Transition.applicand
+  exact ih
+
+
+
+theorem EvalCon.is_value_determines_hole
+  (evalcon : EvalCon E)
+  (isval : Expr.is_value (E e))
+: E = (fun x => x)
+:= by cases evalcon with
+| hole =>
+  simp
+| applicator arg evalcon' =>
+  reduce at isval
+  simp at isval
+| applicand f evalcon' =>
+  reduce at isval
+  simp at isval
+
+
+theorem EvalCon.extract l
+  (evalcon : EvalCon E)
+: EvalCon (fun e => Expr.extract (E e) l)
+:= by unfold Expr.extract; cases evalcon with
+| hole =>
+  simp
+  apply EvalCon.applicand
+  apply EvalCon.hole
+| applicator arg evalcon' =>
+  simp
+  apply EvalCon.applicand
+  exact applicator arg evalcon'
+| applicand f evalcon' =>
+  simp
+  apply EvalCon.applicand
+  exact applicand f evalcon'
+
+theorem EvalCon.project l
+  (evalcon : EvalCon E)
+: EvalCon (fun e => Expr.project (E e) l)
+:= by unfold Expr.project; cases evalcon with
+| hole =>
+  simp
+  apply EvalCon.applicand
+  apply EvalCon.hole
+| applicator arg evalcon' =>
+  simp
+  apply EvalCon.applicand
+  exact applicator arg evalcon'
+| applicand f evalcon' =>
+  simp
+  apply EvalCon.applicand
+  exact applicand f evalcon'
+
+
+
+
+
+
+
+
+end Lang.Dynamic
