dsn/Lang/Dynamic/FinTyping.lean
@@ -1,0 +1,119 @@
+import Lang.Basic
+import Lang.Dynamic.Transition
+import Lang.Dynamic.EvalCon
+import Lang.Dynamic.TransitionStar
+import Lang.Dynamic.Convergent
+import Lang.Dynamic.Divergent
+
+set_option pp.fieldNotation false
+
+namespace Lang.Dynamic
+
+def FinTyping (e : Expr) : Typ → Prop
+| .top => Convergent e ∨ Divergent e
+| .iso l body => FinTyping (.extract e l) body
+| .entry l body => FinTyping (.project e l) body
+| .path left right => ∀ e' , FinTyping e' left → FinTyping (.app e e') right
+| .unio left right => FinTyping e left ∨ FinTyping e right
+| .inter left right => FinTyping e left ∧ FinTyping e right
+| .diff left right => FinTyping e left ∧ ¬ (FinTyping e right)
+| _ => False
+
+
+def Subtyping.Fin (left right : Typ) : Prop :=
+  ∀ e, FinTyping e left → FinTyping e right
+
+
+mutual
+  theorem FinTyping.subject_reduction
+    (transition : Transition e e')
+  : FinTyping e t → FinTyping e' t
+  := by sorry
+
+  theorem FinTyping.subject_expansion
+    (transition : Transition e e')
+  : FinTyping e' t → FinTyping e t
+  := by sorry
+end
+
+
+theorem FinTyping.path_determines_function
+  (typing : FinTyping e (.path antec consq))
+: ∃ f , TransitionStar e (.function f)
+:= by sorry
+
+theorem FinTyping.convergent_or_divergent
+  (typing : FinTyping e t)
+: Convergent e ∨ Divergent e
+:= by cases t with
+| bot =>
+  unfold FinTyping at typing
+  exact False.elim typing
+
+| top =>
+  unfold FinTyping at typing
+  exact typing
+
+| iso label body =>
+  unfold FinTyping at typing
+  have ih := FinTyping.convergent_or_divergent typing
+  cases ih with
+  | inl h =>
+    apply Or.inl
+    apply Convergent.evalcon_reflection
+    { apply EvalCon.extract label .hole }
+    { exact h }
+  | inr h =>
+    apply Or.inr
+    apply Divergent.evalcon_reflection
+    { apply EvalCon.extract label .hole }
+    { exact h }
+
+| entry label body =>
+  unfold FinTyping at typing
+  have ih := FinTyping.convergent_or_divergent typing
+  cases ih with
+  | inl h =>
+    apply Or.inl
+    apply Convergent.evalcon_reflection
+    { apply EvalCon.project label .hole }
+    { exact h }
+  | inr h =>
+    apply Or.inr
+    apply Divergent.evalcon_reflection
+    { apply EvalCon.project label .hole }
+    { exact h }
+
+| path left right =>
+  apply FinTyping.path_determines_function at typing
+  have ⟨f, h0⟩ := typing
+  apply Or.inl
+  unfold Convergent
+  exists (.function f)
+
+
+| unio left right =>
+  unfold FinTyping at typing
+  cases typing with
+  | inl h =>
+    apply FinTyping.convergent_or_divergent h
+  | inr h =>
+    apply FinTyping.convergent_or_divergent h
+
+| inter left right =>
+  unfold FinTyping at typing
+  have ⟨h0,h1⟩ := typing
+  apply FinTyping.convergent_or_divergent h0
+
+| diff left right =>
+  unfold FinTyping at typing
+  have ⟨h0,h1⟩ := typing
+  apply FinTyping.convergent_or_divergent h0
+| _ =>
+  unfold FinTyping at typing
+  exact False.elim typing
+
+
+
+
+end Lang.Dynamic
