dsn/Lang/Dynamic/Transition.lean
@@ -1,0 +1,115 @@
+import Lang.Basic
+
+set_option pp.fieldNotation false
+
+namespace Lang.Dynamic
+
+mutual
+  def List.pattern_match_entry (label : String) (pat : Pat)
+  : List (String × Expr) → Option (List (String × Expr))
+  | .nil => none
+  | (l, e) :: args =>
+    if l == label then
+      (Expr.pattern_match e pat)
+    else
+      List.pattern_match_entry label pat args
+
+  def List.pattern_match_record (args : List (String × Expr))
+  : List (String × Pat) → Option (List (String × Expr))
+  | .nil => some []
+  | (label, pat) :: pats => do
+    if Pat.free_vars pat ∩ ListPat.free_vars pats == [] then
+      let m0 ← List.pattern_match_entry label pat args
+      let m1 ← List.pattern_match_record args pats
+      return (m0 ++ m1)
+    else
+      .none
+
+  def Expr.pattern_match : Expr → Pat → Option (List (String × Expr))
+  | e, (.var id) => some [(id, e)]
+  | (.record r), (.record p) => List.pattern_match_record r p
+  | _, _ => none
+end
+
+mutual
+  def List.pattern_ids : List (String × Pat) → List String
+  | .nil => .nil
+  | (_, p) :: r =>
+    (Pat.ids p) ++ (List.pattern_ids r)
+
+  def Pat.ids : Pat → List String
+  | .var id => [id]
+  | .iso l body => Pat.ids body
+  | .record r => List.pattern_ids r
+end
+
+
+mutual
+  def List.record_sub (m : List (String × Expr)): List (String × Expr) → List (String × Expr)
+  | .nil => .nil
+  | (l, e) :: r =>
+    (l, Expr.sub m e) :: (List.record_sub m r)
+
+  def List.function_sub (m : List (String × Expr)): List (Pat × Expr) → List (Pat × Expr)
+  | .nil => .nil
+  | (p, e) :: f =>
+    let ids := Pat.ids p
+    (p, Expr.sub (remove_all m ids) e) :: (List.function_sub m f)
+
+  def Expr.sub (m : List (String × Expr)): Expr → Expr
+  | .var id => match (find id m) with
+    | .none => (.var id)
+    | .some e => e
+  | .iso l body => .iso l (Expr.sub m body)
+  | .record r => .record (List.record_sub m r)
+  | .function f => .function (List.function_sub m f)
+  | .app ef ea => .app (Expr.sub m ef) (Expr.sub m ea)
+  | .anno e t => .anno (Expr.sub m e) t
+  | .loop e => .loop (Expr.sub m e)
+end
+
+
+
+inductive Transition : Expr → Expr → Prop
+| entry l r :
+  Transition e e' →
+  Transition (Expr.record ((l, e) :: r)) (Expr.record ((l, e') :: r))
+| record :
+  Transition (Expr.record r) (Expr.record r') →
+  v.is_value →
+  Transition (Expr.record ((l, v) :: r)) (Expr.record ((l, v) :: r'))
+| applicator :
+  Transition ef ef' →
+  Transition (.app ef e) (.app ef' e)
+| applicand f e e' :
+  Transition e e' →
+  Transition (.app (.function f) e) (.app (.function f) e')
+| appmatch : ∀ {p e f v m},
+  v.is_value →
+  Expr.pattern_match v p = some m →
+  Transition (.app (.function ((p,e) :: f)) v) (Expr.sub m e)
+| appskip :
+  v.is_value →
+  Expr.pattern_match v p = none →
+  Transition (.app (.function ((p,e) :: f)) v) (.app (.function f) v)
+| anno : ∀ {e t},
+  Transition (.anno  e t) e
+| loopbody :
+  Transition e e' →
+  Transition (.loop e) (.loop e')
+| looppeel : ∀ {id e},
+  Transition
+    (.loop (.function [(.var id, e)]))
+    (Expr.sub [(id, (.loop (.function [(.var id, e)])))] e)
+
+
+
+theorem Transition.deterministic
+  (transition : Transition e e')
+  (transition' : Transition e e'')
+: e' = e''
+:= by sorry
+
+
+
+end Lang.Dynamic
