dsn/Lang/Dynamic/TransitionStar.lean
@@ -1,0 +1,29 @@
+import Lang.Basic
+import Lang.Dynamic.Transition
+import Lang.Dynamic.EvalCon
+
+set_option pp.fieldNotation false
+
+
+namespace Lang.Dynamic
+
+inductive TransitionStar : Expr → Expr → Prop
+| refl e : TransitionStar e e
+| step e e' e'' : Transition e e' → TransitionStar e' e'' → TransitionStar e e''
+
+
+
+theorem TransitionStar.evalcon_preservation
+  (evalcon : EvalCon E)
+  (transition_star : TransitionStar e e')
+: TransitionStar (E e) (E e')
+:= by induction transition_star with
+| refl e =>
+  exact refl (E e)
+| step e e' e'' h0 h1 ih =>
+  apply TransitionStar.step
+  { apply EvalCon.soundness evalcon h0 }
+  { exact ih }
+
+
+end Lang.Dynamic
